compiler/backend/proofs/stack_namesProofScript.sml
@@ -113,7 +113,9 @@ val inst_rename = Q.store_thm("inst_rename",
     simp[find_name_def] ) >>
   CASE_TAC >> fs[assign_def,word_exp_def] >>
   every_case_tac >> fs[LET_THM,word_exp_def,ri_find_name_def,wordSemTheory.num_exp_def] >>
-  rw[] >> fs[] >> rfs[] >> rw[set_var_find_name])
+  rw[] >> fs[] >> rfs[] >> rw[set_var_find_name]
+  \\ every_case_tac \\ fs [wordSemTheory.word_op_def]
+  \\ rw [] \\ fs [] \\ fs [BIJ_DEF,INJ_DEF] \\ res_tac \\ fs [])
 
 val comp_correct = prove(
   ``!p s r t.
